\section{Ley de conservación unidimensional}

\begin{frame}

	\begin{equation*}
		\diffp{u}{t}+
		\diffp{}{x}
		\left[f\left(u\right)\right]
	\end{equation*}
\end{frame}

\section{Ecuación elíptica bidimensional}

\begin{frame}

	Sea $\Omega\subset\mathbb{R}^{2}$.

	\begin{equation*}
		\begin{cases}
			-\nabla\cdot\nabla u+
			\nabla\cdot\left(bu\right)+
			cu=f & \text{en }\Omega. \\
			u\big|_{\partial\Omega}=0.
		\end{cases}
	\end{equation*}

	$f\in L^{2}\left(\Omega\right)$, $b\in C^{1}\left(\Omega\right)$.
	$\forall\left(x,y\right)\in\Omega:c\left(x,y\right)\geq 0$.
	$\forall\left(x,y\right)\in\Omega:\nabla\cdot b\left(x,y\right)\geq 0$.
\end{frame}

% \appendix

% \section{Cálculo}

% Teorema de Taylor unidimensional

% Sea $n\in\mathbb{N}\cup\left\{0\right\}$.
% Si
% \begin{math}
% 	u\in
% 	C^{n+1}\left(\left[a,b\right],\mathbb{R}\right)
% \end{math}
% y $\forall \left\{x,x_{0}\right\}\subset\left[a,b\right]$,
% entonces
% \begin{equation*}
% 	u\left(x\right)=
% 	\sum_{k=0}^{n}
% 	\left[
% 	\frac{{\left(x-x_{0}\right)}^{k}}{k!}
% 	\diff[k]{u}{x}{\bigg|}_{x_{0}}
% 	\right]+
% 	\int_{x_{0}}^{x}
% 	\frac{{\left(x-t\right)}^{n}}{n!}
% 	\diff[n+1]{u}{x}{\bigg|}_{t}\dl t.
% \end{equation*}

% Forma de Lagrange del resto

% $\exists\xi\in\left(x,x_{0}\right)$

% \begin{equation*}
% 	u\left(x\right)=
% 	\sum_{k=0}^{n}
% 	\frac{{\left(x-x_{0}\right)}^{k}}{k!}
% 	\diff[k]{u}{x}{\bigg|}_{x_{0}}+
% 	\frac{{\left(x-x_{0}\right)}^{n+1}}{\left(n+1\right)!}
% 	\diff[n+1]{u}{x}{\bigg|}_{\xi}.
% \end{equation*}

% \nocite{*}
% \printbibliography[title={Referencias},heading=bibintoc]
